added feature for recursive function expansion

smtlink/z3_files/test5.py
@@ -2,7 +2,7 @@ from sys import path
 path.insert(0,"/ubc/cs/home/y/yanpeng/project/ACL2/smtlink/z3_interface")
 from ACL2_translator import to_smt, Q
 s = to_smt()
-A=s.isReal("A")
+var3=s.isReal("var3")
 hypothesis=s.notx(s.lt(A,10))
-conclusion=s.notx(s.lt((lambda var0:s.ifx(False,1,s.times(var0,(lambda var1:s.ifx(False,1,s.times(var1,(lambda var2:s.ifx(False,1,s.times(var2,False)))(s.plus(-1,var1)))))(s.plus(-1,var0)))))(A),20))
+conclusion=s.notx(s.lt((lambda var0:s.ifx(False,1,s.times(var0,(lambda var1:s.ifx(False,1,s.times(var1,(lambda var2:s.ifx(False,1,s.times(var2,var3)))(s.plus(-1,var1)))))(s.plus(-1,var0)))))(A),20))
 s.prove(hypothesis, conclusion)
