smtlink/test-all.lisp
@@ -17,6 +17,23 @@
 ;; 2. if level provided, each function can be expanded
 ;; for that many levels
 
+;; 2014-07-02
+;; add recursive function replacement and type speficication
+;; :hints
+;;   (("Goal"
+;;     :clause-processor
+;;     (my-clause-processor clause
+;; 			 '( (:expand (:functions ((fdco rationalp)
+;;                                                (m integerp)))
+;;                                   (:expansion-level 1))
+;; 			   (:python-file "test")
+;; 			   (:let ())
+;; 			   (:hypothesize ())
+;; 			   (:use ((:type ())
+;; 				  (:hypo ())
+;; 				  (:main ()))))
+;; 			 )))
+
 ;; test cases
 (in-package "ACL2")
 (logic)
@@ -38,7 +55,7 @@
 ;;   (("Goal"
 ;;     :clause-processor
 ;;     (my-clause-processor clause
-;; 			 '( (:expand ((:functions (bar0))
+;; 			 '( (:expand ((:functions ((bar0 rationalp)))
 ;; 				      (:expansion-level 1)))
 ;; 			   (:python-file "test0")
 ;; 			   (:let ())
@@ -63,7 +80,7 @@
 ;;   (("Goal"
 ;;     :clause-processor
 ;;     (my-clause-processor clause
-;; 			 '( (:expand ((:functions (foo1))
+;; 			 '( (:expand ((:functions ((foo1 rationalp)))
 ;; 				      (:expansion-level 1)))
 ;; 			   (:python-file "test1")
 ;; 			   (:let ())
@@ -72,207 +89,219 @@
 ;; 				  (:hypo ())
 ;; 				  (:main ()))))))))
 
-;; test2
-(defun foo2 (x) (+ x 3))
-(defun bar2 (y) (* 2 (foo2 y)))
+;; ;; test2
+;; (defun foo2 (x) (+ x 3))
+;; (defun bar2 (y) (* 2 (foo2 y)))
 
-(defthm test2
-  (implies (and (and (rationalp y))
-		(and (> y 1)))
-	   (> (bar2 (foo2 y)) 12))
-  :hints
-  (("Goal"
-    :clause-processor
-    (my-clause-processor clause
-			 '( (:expand ((:functions (foo2 bar2))
-				      (:expansion-level 1)))
-			    (:python-file "test2")
-			    (:let ())
-			    (:hypothesize ())
-			    (:use ((:type ())
-				   (:hypo ())
-				   (:main ()))))))))
-
-;; test3
-(defun foo3 (x args) (+ x (nth 0 args) (nth 1 args)))
-
-(defthm test3
-  (implies (and (and (rationalp x)
-		     (integerp i)
-		     (integerp j))
-		(and (> x 0)
-		     (> i 0)
-		     (> j 0)))
-	   (> (foo3 x '(i j)) 0))
-  :hints
-  (("Goal"
-    :clause-processor
-    (my-clause-processor clause
-			 '( (:expand ((:functions (foo3))
-				      (:expansion-level 1)))
-			    (:python-file "test3")
-			    (:let ())
-			    (:hypothesize ())
-			    (:use ((:type ())
-				   (:hypo ())
-				   (:main ()))))))))
-
-;; test4
-;; x^2 + y^2 >= 2xy
-;; a(x,y) = x*y
-;; b(x) = 2*x = (a 2 x)
-;; c(x,y) = x+y
-;; d(x) = x^2 = (a x x)
-;; e(x) = -x
-;; f(x,y) = x-y = (c x -y) = (c x (e y))
-(defun a4 (x y) (* x y))
-(defun b4 (x) (a4 2 x))
-(defun c4 (x y) (+ x y))
-(defun d4 (x) (a4 x x))
-(defun e4 (x) (- x))
-(defun f4 (x y) (c4 x (e4 y)))
-
-(defthm test4
-    (implies (and (and (rationalp a)
-		       (rationalp b))
-		  (and))
-	     (>= (f4 (d4 (c4 a b))
-		     (a4 (b4 a) b))
-		 (a4 (b4 a) b)))
-  :hints
-  (("Goal"
-    :clause-processor
-    (my-clause-processor clause
-			 '( (:expand ((:functions (a4 b4 c4 d4 e4 f4)))
-			             ;;(:expansion-level 1)
-			     )
-			    (:python-file "test4")
-			    (:let ())
-			    (:hypothesize ())
-			    (:use ((:type ())
-				   (:hypo ())
-				   (:main ()))))))))
-
-;; ;; test5: with recursive call
-;; ;; (fac)
-;; (defun fac (x) (if (zp x) 1 (* x (fac (1- x)))))
-
-;; (defthm test5
-;;     (implies (and (and (integerp a))
-;; 		  (and (>= a 10)))
-;; 	     (>= (fac a) 20))
+;; (defthm test2
+;;   (implies (and (and (rationalp y))
+;; 		(and (> y 1)))
+;; 	   (> (bar2 (foo2 y)) 12))
 ;;   :hints
 ;;   (("Goal"
 ;;     :clause-processor
 ;;     (my-clause-processor clause
-;; 			 '( (:expand ((:functions (fac))
-;; 				      (:expansion-level 3)))
-;; 			    (:python-file "test5")
+;; 			 '( (:expand ((:functions ((foo2 rationalp)
+;; 						   (bar2 rationalp)))
+;; 				      (:expansion-level 1)))
+;; 			    (:python-file "test2")
 ;; 			    (:let ())
 ;; 			    (:hypothesize ())
-;;                          (:use ((:type ())
-;;                                 (:hypo ())
-;;                                 (:main ()))))))))
+;; 			    (:use ((:type ())
+;; 				   (:hypo ())
+;; 				   (:main ()))))))))
 
+;; ;; test3
+;; (defun foo3 (x args) (+ x (nth 0 args) (nth 1 args)))
 
-;; test6: user given hypothesis
-;; a - real
-;; b - real
-;; gamma - real
-;; m - integer
-;; n - integer
-;; 0 < gamma < 1
-;; 0 < m < n
-;; adapted from test4: a^2 + b^2 >= 2ab
+;; (defthm test3
+;;   (implies (and (and (rationalp x)
+;; 		     (integerp i)
+;; 		     (integerp j))
+;; 		(and (> x 0)
+;; 		     (> i 0)
+;; 		     (> j 0)))
+;; 	   (> (foo3 x '(i j)) 0))
+;;   :hints
+;;   (("Goal"
+;;     :clause-processor
+;;     (my-clause-processor clause
+;; 			 '( (:expand ((:functions ((foo3 rationalp)))
+;; 				      (:expansion-level 1)))
+;; 			    (:python-file "test3")
+;; 			    (:let ())
+;; 			    (:hypothesize ())
+;; 			    (:use ((:type ())
+;; 				   (:hypo ())
+;; 				   (:main ()))))))))
 
-;; 2*a*b*gamma^n <= -2*a*b*gamma^m + ...???
-(defun a6 (x y) (* x y))
-(defun b6 (x) (a6 2 x))
-(defun c6 (x y) (+ x y))
-(defun d6 (x) (a6 x x))
-(defun e6 (x) (- x))
-(defun f6 (x y) (c6 x (e6 y)))
-(defun foo6 (x n) (expt x n))
+;; ;; test4
+;; ;; x^2 + y^2 >= 2xy
+;; ;; a(x,y) = x*y
+;; ;; b(x) = 2*x = (a 2 x)
+;; ;; c(x,y) = x+y
+;; ;; d(x) = x^2 = (a x x)
+;; ;; e(x) = -x
+;; ;; f(x,y) = x-y = (c x -y) = (c x (e y))
+;; (defun a4 (x y) (* x y))
+;; (defun b4 (x) (a4 2 x))
+;; (defun c4 (x y) (+ x y))
+;; (defun d4 (x) (a4 x x))
+;; (defun e4 (x) (- x))
+;; (defun f4 (x y) (c4 x (e4 y)))
 
-(defthm test6
-    (implies (and (and (rationalp a)
-		       (rationalp b)
-		       (rationalp gamma)
-		       (integerp m)
-		       (integerp n))
-		  (and (> gamma 0)
-		       (< gamma 1)
-		       (> m 0)
-		       (< m n)))
-	     (>= (a6 (expt gamma m)
-		    (f6 (d6 (c6 a b))
-			(a6 (b6 a) b)))
-		 (a6 (foo6 gamma n)
-		    (a6 (b6 a) b))))
+;; (defthm test4
+;;     (implies (and (and (rationalp a)
+;; 		       (rationalp b))
+;; 		  (and))
+;; 	     (>= (f4 (d4 (c4 a b))
+;; 		     (a4 (b4 a) b))
+;; 		 (a4 (b4 a) b)))
+;;   :hints
+;;   (("Goal"
+;;     :clause-processor
+;;     (my-clause-processor clause
+;; 			 '( (:expand ((:functions ((a4 rationalp)
+;; 						   (b4 rationalp)
+;; 						   (c4 rationalp)
+;; 						   (d4 rationalp)
+;; 						   (e4 rationalp)
+;; 						   (f4 rationalp))))
+;; 			             ;;(:expansion-level 1)
+;; 			     )
+;; 			    (:python-file "test4")
+;; 			    (:let ())
+;; 			    (:hypothesize ())
+;; 			    (:use ((:type ())
+;; 				   (:hypo ())
+;; 				   (:main ()))))))))
+
+;; test5: with recursive call
+;; (fac)
+(defun fac (x) (if (zp x) 1 (* x (fac (1- x)))))
+
+(defthm test5
+    (implies (and (and (integerp a))
+		  (and (>= a 10)))
+	     (>= (fac a) 20))
   :hints
   (("Goal"
     :clause-processor
     (my-clause-processor clause
-			 '( (:expand ((:functions (a6 b6 c6 d6 e6 f6 foo6))
-				      (:expansion-level 1)))
-			    (:python-file "test6")
-			    (:let ((expt_gamma_m (expt gamma m) rationalp)
-				   (expt_gamma_n (expt gamma n) rationalp)))
-			    (:hypothesize ((< expt_gamma_n expt_gamma_m)
-					   (> expt_gamma_m 0)
-					   (> expt_gamma_n 0)))
-			    (:use ((:type ())
-				   (:hypo ())
-				   (:main ()))))))))
+			 '( (:expand ((:functions ((fac integerp)))
+				      (:expansion-level 3)))
+			    (:python-file "test5")
+			    (:let ())
+			    (:hypothesize ())
+                         (:use ((:type ())
+                                (:hypo ())
+                                (:main ()))))))))
 
-;; test7: user given hints
-;; Design:
-;; '( (:expand (...))
-;;    (:python-file "..")
-;;    (:let ((...)
-;;           (...)))
-;;    (:hypothesis ((...)
-;;                  (...)))
-;;    (:use (:type ((...) (...) (...)))
-;;          (:hypo ((...) (...) (...)))
-;;          (:main ((...) (...) (...)))))
-;; Explanation:
-;; The three classes of hints are seperately for types,
-;; hypotheses and the main theorem returned.
-;; Type theorems come from the type statements in let
-;; bindings, hypo theorems come from user provided hypotheses,
-;; and the main theorem is the implication from SMT result
-;; to the initial theorem we want to prove.
-;; Note:
-;; Each theorem can have multiple hints.
-;; 
 
-(defthm hint-thm-7-1
-  (implies (and (rationalp x)
-		(rationalp y))
-	   (>= (* (+ x y) (+ x y)) 0))
-  :rule-classes :linear)
+;; ;; test6: user given hypothesis
+;; ;; a - real
+;; ;; b - real
+;; ;; gamma - real
+;; ;; m - integer
+;; ;; n - integer
+;; ;; 0 < gamma < 1
+;; ;; 0 < m < n
+;; ;; adapted from test4: a^2 + b^2 >= 2ab
 
-;; (defthm hint-thm-7-2
+;; ;; 2*a*b*gamma^n <= -2*a*b*gamma^m + ...???
+;; (defun a6 (x y) (* x y))
+;; (defun b6 (x) (a6 2 x))
+;; (defun c6 (x y) (+ x y))
+;; (defun d6 (x) (a6 x x))
+;; (defun e6 (x) (- x))
+;; (defun f6 (x y) (c6 x (e6 y)))
+;; (defun foo6 (x n) (expt x n))
+
+;; (defthm test6
+;;     (implies (and (and (rationalp a)
+;; 		       (rationalp b)
+;; 		       (rationalp gamma)
+;; 		       (integerp m)
+;; 		       (integerp n))
+;; 		  (and (> gamma 0)
+;; 		       (< gamma 1)
+;; 		       (> m 0)
+;; 		       (< m n)))
+;; 	     (>= (a6 (expt gamma m)
+;; 		    (f6 (d6 (c6 a b))
+;; 			(a6 (b6 a) b)))
+;; 		 (a6 (foo6 gamma n)
+;; 		    (a6 (b6 a) b))))
+;;   :hints
+;;   (("Goal"
+;;     :clause-processor
+;;     (my-clause-processor clause
+;; 			 '( (:expand ((:functions ((a6 rationalp)
+;; 						   (b6 rationalp)
+;; 						   (c6 rationalp)
+;; 						   (d6 rationalp)
+;; 						   (e6 rationalp)
+;; 						   (f6 rationalp)
+;; 						   (foo6 rationalp))))
+;; 				      (:expansion-level 1)))
+;; 			    (:python-file "test6")
+;; 			    (:let ((expt_gamma_m (expt gamma m) rationalp)
+;; 				   (expt_gamma_n (expt gamma n) rationalp)))
+;; 			    (:hypothesize ((< expt_gamma_n expt_gamma_m)
+;; 					   (> expt_gamma_m 0)
+;; 					   (> expt_gamma_n 0)))
+;; 			    (:use ((:type ())
+;; 				   (:hypo ())
+;; 				   (:main ()))))))))
+
+;; ;; test7: user given hints
+;; ;; Design:
+;; ;; '( (:expand (...))
+;; ;;    (:python-file "..")
+;; ;;    (:let ((...)
+;; ;;           (...)))
+;; ;;    (:hypothesis ((...)
+;; ;;                  (...)))
+;; ;;    (:use (:type ((...) (...) (...)))
+;; ;;          (:hypo ((...) (...) (...)))
+;; ;;          (:main ((...) (...) (...)))))
+;; ;; Explanation:
+;; ;; The three classes of hints are seperately for types,
+;; ;; hypotheses and the main theorem returned.
+;; ;; Type theorems come from the type statements in let
+;; ;; bindings, hypo theorems come from user provided hypotheses,
+;; ;; and the main theorem is the implication from SMT result
+;; ;; to the initial theorem we want to prove.
+;; ;; Note:
+;; ;; Each theorem can have multiple hints.
+;; ;; 
+
+;; (defthm hint-thm-7-1
 ;;   (implies (and (rationalp x)
 ;; 		(rationalp y))
-;; 	   (equal (* (+ x y) (+ x y))
-;; 		  (expt (+ x y) 2))))
+;; 	   (>= (* (+ x y) (+ x y)) 0))
+;;   :rule-classes :linear)
 
-(defthm test7
-  (implies (and (and (rationalp x)
-		     (rationalp y))
-		(and))
-	   (>= (expt (+ x y) 2) 0))
-  :hints
-  (("Goal"
-    :clause-processor
-    (my-clause-processor clause
-			 '( (:expand ())
-			    (:python-file "test7")
-			    (:let ((expt_plus_x_y_square (expt (+ x y) 2) rationalp)))
-			    (:hypothesize ((>= expt_plus_x_y_square 0)))
-			    (:use ((:type ())
-			    	   (:hypo ((hint-thm-7-1)))
-			    	   (:main (hint-thm-7-1))))
-			   )))))
+;; ;; (defthm hint-thm-7-2
+;; ;;   (implies (and (rationalp x)
+;; ;; 		(rationalp y))
+;; ;; 	   (equal (* (+ x y) (+ x y))
+;; ;; 		  (expt (+ x y) 2))))
+
+;; (defthm test7
+;;   (implies (and (and (rationalp x)
+;; 		     (rationalp y))
+;; 		(and))
+;; 	   (>= (expt (+ x y) 2) 0))
+;;   :hints
+;;   (("Goal"
+;;     :clause-processor
+;;     (my-clause-processor clause
+;; 			 '( (:expand ())
+;; 			    (:python-file "test7")
+;; 			    (:let ((expt_plus_x_y_square (expt (+ x y) 2) rationalp)))
+;; 			    (:hypothesize ((>= expt_plus_x_y_square 0)))
+;; 			    (:use ((:type ())
+;; 			    	   (:hypo ((hint-thm-7-1)))
+;; 			    	   (:main (hint-thm-7-1))))
+;; 			   )))))
